# 尼科彻斯定理
https://www.nowcoder.com/practice/dbace3a5b3c4480e86ee3277f3fe1e85

    import java.util.Scanner;
    
    // 注意类名必须为 Main, 不要有任何 package xxx 信息
    public class Main {
        /**
         * 输入m
         * 起始数n
         * 
         * n+(n+2)+(n+4)+...+(n+2*(m-1)) = m^3
         * n*m+(2+4+...+2*(m-1)) = m^3
         * n*m+[(2+2*(m-1))*(m-1)]/2 = m^3
         * n*m+m*(m-1) = m^3
         * n+(m-1) = m^2
         * n = m^2 - (m-1) = m^2-m+1
         * @param args
         */
        public static void main(String[] args) {
            Scanner in = new Scanner(System.in);
    
            while (in.hasNextInt()){
                int m = in.nextInt();
    
                int n = (int)(Math.pow(m, 2)-m+1);
    
                for(int i=1; i<m; i++){
                    System.out.print(n+"+");
                    n += 2;
                }
                System.out.print(n);
            }
        }
    }
    

